---
title: "GRADUATE STUDENT STAT 840 A2"
author: "Vsevolod Ladtchenko 20895137"
output: pdf_document
---

```{r setup, include=FALSE}
knitr::opts_chunk$set(echo = TRUE)
```

# Problem 6

## a)

$$
\begin{aligned}
\pi (\theta \mid \mathbb{X}) &\propto f(\mathbb{X} \mid \theta) \pi(\theta) \\
\pi (\alpha, \eta \mid \mathbb{X}) &\propto f(\mathbb{X} \mid \alpha, \eta) \pi(\alpha, \eta) \\
f(x \mid \alpha,  \eta) &\propto \alpha \eta x^{\alpha - 1} e^{-\eta x^{\alpha}} \\
f(\mathbb{X} \mid \alpha,  \eta) &= \prod_{i=1}^n f(x_i \mid \alpha,  \eta) \\
&\propto \prod_{i=1}^n \alpha \eta x_i^{\alpha - 1} e^{-\eta x_i^{\alpha}} \\
&\propto \alpha^n \eta^n \prod_{i=1}^n x_i^{\alpha - 1} e^{-\eta x_i^{\alpha}} \\
\pi(\alpha, \eta) &\propto e^{-\alpha} \eta^{\beta - 1} e^{-c \eta} \\
&\propto e^{-\alpha -c \eta} \eta^{\beta - 1} \\
\pi (\alpha, \eta \mid \mathbb{X}) &\propto e^{-\alpha -c \eta} \eta^{\beta - 1} \alpha^n \eta^n \prod_{i=1}^n x_i^{\alpha - 1} e^{-\eta x_i^{\alpha}} \\
&\propto e^{-\alpha -c \eta} \eta^{n + \beta - 1} \alpha^n \prod_{i=1}^n x_i^{\alpha - 1} e^{-\eta x_i^{\alpha}} \\
\end{aligned}
$$

```{R}
log_post_pi = function(alp, eta, x, c,b)
{
  n = length(x)
  p1 = (-alp - c*eta)
  p2 = (n+b-1)*log(eta)
  p3 = n*log(alp)
  p4 = (alp-1)*log(x) + (-eta * x^alp)
  return(p1 + p2 + p3 + sum(p4))
}

post_pi = function(alp, eta, x, c,b)
{
  n = length(x)
  p1 = exp(-alp - c*eta)
  p2 = eta^(n+b-1)
  p3 = alp^n
  p4 = x^(alp-1) * exp(-eta * x^alp)
  return(p1 * p2 * p3 * prod(p4))
}

q = function(a2,n2,a1,n1)
{
  p1 = 1 / (a1 * n1)
  p2 = exp(-a2/a1 -n2/n1)
  return(p1*p2)
}
```


## b)

$$
\begin{aligned}
\alpha( \theta_n, \theta^*) &= \min \biggl\{ \frac{\pi(\theta^* \mid \mathbb{X}) q(\theta^*, \theta_n)}{\pi(\theta_n \mid \mathbb{X}) q(\theta_n, \theta^*)}, 1 \biggr\} \qquad \texttt{notes 4 p 19}\\
\rho(\alpha^*, \eta^*  \mid \alpha_{(t)}, \eta_{(t)} ) &= \min \biggl\{ \frac{\pi(\alpha^*, \eta^* \mid \mathbb{X}) q(\alpha^*, \eta^* \mid \alpha_{(t)}, \eta_{(t)})}{\pi(\alpha_{(t)}, \eta_{(t)} \mid \mathbb{X}) q(\alpha_{(t)}, \eta_{(t)} \mid \alpha^*, \eta^*)}, 1 \biggr\} \\
\pi (\alpha^*, \eta^* \mid \mathbb{X}) &\propto e^{-\alpha^* -c \eta^*} \eta^{* n + \beta - 1} \alpha^{*n} \prod_{i=1}^n x_i^{\alpha^* - 1} e^{-\eta^* x_i^{\alpha^*}} \\
\pi (\alpha_{(t)}, \eta_{(t)} \mid \mathbb{X}) &\propto e^{-\alpha_{(t)} -c \eta_{(t)}} \eta_{(t)}^{n + \beta - 1} \alpha_{(t)}^n \prod_{i=1}^n x_i^{\alpha_{(t)} - 1} e^{-\eta_{(t)} x_i^{\alpha_{(t)}}} \\
\frac{\pi (\alpha^*, \eta^* \mid \mathbb{X})}{\pi (\alpha_{(t)}, \eta_{(t)} \mid \mathbb{X}) } &= \frac{e^{-\alpha^* -c \eta^*} \eta^{* n + \beta - 1} \alpha^{*n} \prod_{i=1}^n x_i^{\alpha^* - 1} e^{-\eta^* x_i^{\alpha^*}}}{e^{-\alpha_{(t)} -c \eta_{(t)}} \eta_{(t)}^{n + \beta - 1} \alpha_{(t)}^n \prod_{i=1}^n x_i^{\alpha_{(t)} - 1} e^{-\eta_{(t)} x_i^{\alpha_{(t)}}}} \\
&= e^{\alpha_{(t)} +c \eta_{(t)} -\alpha^* -c \eta^*} \frac{ \eta^{* n + \beta - 1} \alpha^{*n} \prod_{i=1}^n x_i^{\alpha^* - 1} e^{-\eta^* x_i^{\alpha^*}}}{ \eta_{(t)}^{n + \beta - 1} \alpha_{(t)}^n \prod_{i=1}^n x_i^{\alpha_{(t)} - 1} e^{-\eta_{(t)} x_i^{\alpha_{(t)}}}} \\
&= e^{\alpha_{(t)} +c \eta_{(t)} -\alpha^* -c \eta^*} \frac{ \eta^{* n + \beta - 1} \alpha^{*n} }{ \eta_{(t)}^{n + \beta - 1} \alpha_{(t)}^n } \prod_{i=1}^n x_i^{\alpha^*-\alpha_{(t)}} e^{\eta_{(t)} x_i^{\alpha_{(t)}}-\eta^* x_i^{\alpha^*}} \\
q(\alpha^*, \eta^* \mid \alpha_{(t)}, \eta_{(t)}) &= \frac{1}{\alpha_{(t)} \eta_{(t)}} \exp \biggl\{ - \frac{\alpha^*}{\alpha_{(t)}} - \frac{\eta^*}{\eta_{(t)}} \biggr\} \\
q(\alpha_{(t)}, \eta_{(t)} \mid \alpha^*, \eta^*) &= \frac{1}{\alpha^* \eta^*} \exp \biggl\{ - \frac{\alpha_{(t)}}{\alpha^*} - \frac{\eta_{(t)}}{\eta^*} \biggr\}\\
\frac{q(\alpha^*, \eta^* \mid \alpha_{(t)}, \eta_{(t)})}{q(\alpha_{(t)}, \eta_{(t)} \mid \alpha^*, \eta^*)} &= \frac{\alpha^* \eta^*}{\alpha_{(t)} \eta_{(t)}} \exp \biggl\{ - \frac{\alpha^*}{\alpha_{(t)}} - \frac{\eta^*}{\eta_{(t)}} + \frac{\alpha_{(t)}}{\alpha^*} + \frac{\eta_{(t)}}{\eta^*} \biggr\} \\
&= \frac{\alpha^* \eta^*}{\alpha_{(t)} \eta_{(t)}} e^{ - \frac{\alpha^*}{\alpha_{(t)}} - \frac{\eta^*}{\eta_{(t)}} + \frac{\alpha_{(t)}}{\alpha^*} + \frac{\eta_{(t)}}{\eta^*}} \\
\rho(\alpha^*, \eta^*  \mid \alpha_{(t)}, \eta_{(t)} ) &= \min \biggl\{ \frac{\alpha^* \eta^*}{\alpha_{(t)} \eta_{(t)}} e^{ - \frac{\alpha^*}{\alpha_{(t)}} - \frac{\eta^*}{\eta_{(t)}} + \frac{\alpha_{(t)}}{\alpha^*} + \frac{\eta_{(t)}}{\eta^*}  +\alpha_{(t)} +c \eta_{(t)} -\alpha^* -c \eta^*} \frac{ \eta^{* n + \beta - 1} \alpha^{*n} }{ \eta_{(t)}^{n + \beta - 1} \alpha_{(t)}^n } \prod_{i=1}^n x_i^{\alpha^*-\alpha_{(t)}} e^{\eta_{(t)} x_i^{\alpha_{(t)}}-\eta^* x_i^{\alpha^*}}, 1 \biggr\} \\
&= \min \biggl\{ e^{ - \frac{\alpha^*}{\alpha_{(t)}} - \frac{\eta^*}{\eta_{(t)}} + \frac{\alpha_{(t)}}{\alpha^*} + \frac{\eta_{(t)}}{\eta^*}  +\alpha_{(t)} +c \eta_{(t)} -\alpha^* -c \eta^*} \frac{ \eta^{* n + \beta} \alpha^{*n+1} }{ \eta_{(t)}^{n + \beta} \alpha_{(t)}^{n+1} } \prod_{i=1}^n x_i^{\alpha^*-\alpha_{(t)}} e^{\eta_{(t)} x_i^{\alpha_{(t)}}-\eta^* x_i^{\alpha^*}}, 1 \biggr\} \\
\end{aligned}
$$

## c)

How to generate the chain:

1. initialize $n = 0$ and $\alpha_n, \eta_n$

2. sample $\alpha^*, \eta^*$ from $q(\alpha^*, \eta^* \mid \alpha_n, \eta_n)$, $u$ from $U(0,1)$

3. if $u \leq \rho(\alpha^*, \eta^*  \mid \alpha_n, \eta_n )$ then set $\alpha_{n+1} = \alpha^*$ and $\eta_{n+1} = \eta^*$, else $\alpha_{n+1} = \alpha_n$ and $\eta_{n+1} = \eta_n$

4. set $n = n + 1$ and goto step 2.

```{R, error = TRUE}
p = function(as, at, ns, nt, c, b, n, x)
{
  p1 = exp(-as/at -ns/nt +at/as + nt/ns +at +c*nt -as -c*ns)
  p2 = (ns/nt)^(n+b) * (as/at)^(n+1)
  p3 = prod(x^(as-at) * exp(nt*x^at - ns * x^as))
  return(min(p1*p2*p3, 1))
}

run = function(x,len,c,b)
{
  NN = 1000
  alp_n = rep(NA,NN)
  eta_n = rep(NA,NN)
  
  # step 1
  alp_n[1] = 1 # initial alpha
  eta_n[1] = 1 # initial eta 
  
  for (i in 2:NN)
  {
    alpha = alp_n[i-1]
    eta = eta_n[i-1]
    
    # step 2
    alpha_star = rexp(1, 1/alpha)
    eta_star = rexp(1, 1/eta)
    u = runif(1)
    
    # step 3
    if (u <= p(alpha_star, alpha, eta_star, eta, c, b, len, x))
    {
      alp_n[i] = alpha_star
      eta_n[i] = eta_star
    } else 
    {
      alp_n[i] = alpha
      eta_n[i] = eta
    }
  }
  
  par(mfrow=c(3,2))
  hist(alp_n)
  hist(eta_n)
  plot(alp_n, type='l')
  plot(eta_n, type='l')
  acf(alp_n)
  acf(eta_n)
}

# hyper params
x = c(0.56, 2.26, 1.90, 0.94, 1.40, 1.39, 1.00, 1.45, 2.32, 2.08, 0.89, 1.68)
len = length(x)

run(x,len,c=0.1,b=1)
run(x,len,c=4,b=1)
run(x,len,c=4,b=0.1)
run(x,len,c=10,b=0.1)
run(x,len,c=0.1,b=0.1)
run(x,len,c=0.1,b=4)
run(x,len,c=0.1,b=10)
```

## d + e)

```{R, error = TRUE}
NN = 1000
alp_n = rep(NA,NN)
eta_n = rep(NA,NN)

# step 1
alp_n[1] = 1 # initial alpha
eta_n[1] = 1 # initial eta 

for (i in 2:NN)
{
  alpha = alp_n[i-1]
  eta = eta_n[i-1]
  
  # step 2
  alpha_star = rexp(1, 1/alpha)
  eta_star = rexp(1, 1/eta)
  u = runif(1)
  
  # step 3
  if (u <= p(alpha_star, alpha, eta_star, eta, c, b, len, x))
  {
    alp_n[i] = alpha_star
    eta_n[i] = eta_star
  } else 
  {
    alp_n[i] = alpha
    eta_n[i] = eta
  }
}

mean(alp_n)

mean(eta_n)

quantile(alp_n, probs = c(0.025, 0.975)) 

quantile(eta_n, probs = c(0.025, 0.975)) 


post_pi = function(alp, eta)
{
  n = length(x)
  p1 = exp(-alp - c*eta)
  p2 = eta^(n+b-1)
  p3 = alp^n
  p4 = x^(alp-1) * exp(-eta * x^alp)
  return(p1 * p2 * p3 * prod(p4))
}

max(post_pi(alp_n))

```
